isa/Halicore_Type_Meaning.thy
@@ -26,7 +26,6 @@ definition Uforall :: "(U \<rightarrow> U) \<rightarrow> U"
   where "Uforall = (\<Lambda> f. Udefl\<cdot>(T_abs\<cdot>(defl_fun1 (fup\<cdot>Vtfun) (V_case\<cdot>\<bottom>\<cdot>\<bottom>\<cdot>\<bottom>\<cdot>up\<cdot>\<bottom>) u_map\<cdot>(pi_defl\<cdot>ID_defl\<cdot>(\<Lambda> u. T_rep\<cdot>(of_U\<cdot>(f\<cdot>u)))))))"
 
 primrec ty_denote :: "(nat \<Rightarrow> U) \<Rightarrow> ty \<Rightarrow> U"
-  and tdef_denote :: "(nat \<Rightarrow> U) \<Rightarrow> tdef \<Rightarrow> U"
   and cons_denote :: "(nat \<Rightarrow> U) \<Rightarrow> ty list list \<Rightarrow> T list list"
   and args_denote :: "(nat \<Rightarrow> U) \<Rightarrow> ty list \<Rightarrow> T list"
 where ty_denote_TyVar:
@@ -39,15 +38,15 @@ where ty_denote_TyVar:
   | ty_denote_TyAll:
     "ty_denote \<sigma> (TyAll k t) =
       Uforall\<cdot>(\<Lambda> u. ty_denote (nat_case u \<sigma>) t)"
+  | ty_denote_TyLam:
+    "ty_denote \<sigma> (TyLam k t) =
+      Ufun\<cdot>(\<Lambda> x. ty_denote (nat_case x \<sigma>) t)" (* FIXME: don't ignore k *)
+  | ty_denote_TyFix:
+    "ty_denote \<sigma> (TyFix k t) = (\<mu> x. ty_denote (nat_case x \<sigma>) t)"
   | ty_denote_TyRec:
-    "ty_denote \<sigma> (TyRec d) = (\<mu> x. tdef_denote (nat_case x \<sigma>) d)"
-  | tdef_denote_TyLam:
-    "tdef_denote \<sigma> (TyLam k d) =
-      Ufun\<cdot>(\<Lambda> x. tdef_denote (nat_case x \<sigma>) d)" (* FIXME: don't ignore k *)
-  | tdef_denote_TyNew:
-    "tdef_denote \<sigma> (TyNew t) = ty_denote \<sigma> t"
-  | tdef_denote_TyData:
-    "tdef_denote \<sigma> (TyData s tss) = to_U\<cdot>(Tdata'\<cdot>s\<cdot>(cons_denote \<sigma> tss))"
+    "ty_denote \<sigma> (TyRec k t) = (\<mu> x. ty_denote (nat_case x \<sigma>) t)"
+  | ty_denote_TyData:
+    "ty_denote \<sigma> (TyData s tss) = to_U\<cdot>(Tdata'\<cdot>s\<cdot>(cons_denote \<sigma> tss))"
   | cons_denote_Nil:
     "cons_denote \<sigma> [] = []"
   | cons_denote_Cons:
@@ -67,10 +66,9 @@ done
 
 lemma
   shows cont_ty_denote: "cont (\<lambda>\<sigma>. ty_denote \<sigma> t)"
-  and cont_tdef_denote: "cont (\<lambda>\<sigma>. tdef_denote \<sigma> d)"
   and cont_cons_denote: "cont (\<lambda>\<sigma>. cons_denote \<sigma> tss)"
   and cont_args_denote: "cont (\<lambda>\<sigma>. args_denote \<sigma> ts)"
-apply (induct t and d and tss and ts)
+apply (induct t and tss and ts)
 txt "TyVar"
 apply (simp, rule cont_fun)
 txt "TyBase"
@@ -81,16 +79,19 @@ txt "TyAll"
 apply simp
 apply (intro cont2cont)
 apply (erule cont_compose, simp)
-txt "TyRec"
-apply simp
-apply (intro cont2cont)
-apply (erule cont_compose, simp)
 txt "TyLam"
 apply simp
 apply (intro cont2cont)
 apply (erule cont_compose, simp)
+txt "TyFix"
+apply simp
+apply (intro cont2cont)
+apply (erule cont_compose, simp)
+txt "TyRec"
+apply simp
+apply (intro cont2cont)
+apply (erule cont_compose, simp)
 
-apply simp (* TyNew *)
 apply simp (* TyData *)
 apply simp (* [] *)
 apply simp (* ts # tss *)
@@ -99,7 +100,6 @@ apply simp (* t # ts *)
 done
 
 declare cont_ty_denote [THEN cont_compose, simp, cont2cont]
-declare cont_tdef_denote [THEN cont_compose, simp, cont2cont]
 
 lemma nat_case_substVar [simp]:
   "nat_case u (substVar \<sigma> i x) = substVar (nat_case u \<sigma>) (Suc i) x"
@@ -108,13 +108,11 @@ by (rule ext, rename_tac n, case_tac n, simp_all)
 lemma
   shows ty_denote_ty_lift:
     "ty_denote (substVar \<sigma> i y) (ty_lift i t) = ty_denote \<sigma> t"
-  and tdef_denote_tdef_lift:
-    "tdef_denote (substVar \<sigma> i y) (tdef_lift i d) = tdef_denote \<sigma> d"
   and cons_denote_cons_lift:
     "cons_denote (substVar \<sigma> i y) (cons_lift i tss) = cons_denote \<sigma> tss"
   and args_denote_args_lift:
     "args_denote (substVar \<sigma> i y) (args_lift i ts) = args_denote \<sigma> ts"
-by (induct t and d and tss and ts arbitrary: \<sigma> i and \<sigma> i and \<sigma> i and \<sigma> i)
+by (induct t and tss and ts arbitrary: \<sigma> i and \<sigma> i and \<sigma> i)
   simp_all
 
 lemma substVar_0: "substVar \<sigma> 0 x = nat_case x \<sigma>"
@@ -127,27 +125,24 @@ lemma
   shows ty_denote_ty_subst:
     "ty_denote \<sigma> (ty_subst i t x) =
      ty_denote (substVar \<sigma> i (ty_denote \<sigma> x)) t"
-  and tdef_denote_tdef_subst:
-    "tdef_denote \<sigma> (tdef_subst i d x) =
-     tdef_denote (substVar \<sigma> i (ty_denote \<sigma> x)) d"
   and cons_denote_cons_subst:
     "cons_denote \<sigma> (cons_subst i tss x) =
      cons_denote (substVar \<sigma> i (ty_denote \<sigma> x)) tss"
   and args_denote_args_subst:
     "args_denote \<sigma> (args_subst i ts x) =
      args_denote (substVar \<sigma> i (ty_denote \<sigma> x)) ts"
-apply (induct t and d and tss and ts
-  arbitrary: \<sigma> i x and \<sigma> i x and \<sigma> i x and \<sigma> i x)
+apply (induct t and tss and ts arbitrary: \<sigma> i x and \<sigma> i x and \<sigma> i x)
 apply (simp add: substVar_def) (* TyVar *)
 apply simp (* TyBase *)
 apply simp (* TyApp *)
 txt "TyAll"
 apply (simp add: ty_denote_ty_lift [where i=0, unfolded substVar_0])
-txt "TyRec"
-apply (simp add: ty_denote_ty_lift [where i=0, unfolded substVar_0])
 txt "TyLam"
 apply (simp add: ty_denote_ty_lift [where i=0, unfolded substVar_0])
-apply simp (* TyNew *)
+txt "TyFix"
+apply (simp add: ty_denote_ty_lift [where i=0, unfolded substVar_0])
+txt "TyRec"
+apply (simp add: ty_denote_ty_lift [where i=0, unfolded substVar_0])
 apply simp (* TyData *)
 apply simp (* [] *)
 apply simp (* ts # tss *)
@@ -155,25 +150,34 @@ apply simp (* [] *)
 apply simp (* t # ts *)
 done
 
-lemma ty_ax_ty_denote:
-  "ty_ax \<Gamma> t d k \<Longrightarrow> ty_denote \<sigma> t = tdef_denote \<sigma> d"
-apply (induct set: ty_ax)
-txt "TyRec"
-apply (simp add: tdef_denote_tdef_subst substVar_0)
+lemma step_ty_denote:
+  "step t u \<Longrightarrow> ty_denote \<sigma> t = ty_denote \<sigma> u"
+apply (induct arbitrary: \<sigma> set: step)
+txt "unfold"
+apply (simp add: ty_denote_ty_subst substVar_0)
 apply (subst fix_eq, simp)
-txt "TyApp"
-apply (simp add: tdef_denote_tdef_subst substVar_0)
+txt "beta"
+apply (simp add: ty_denote_ty_subst substVar_0)
+txt "etc"
+apply simp_all
+txt "TyData"
+apply (rule cfun_arg_cong)
+apply (erule list_all2_induct, simp)
+apply (erule list_all2_induct, simp, simp)
 done
 
-lemma ty_eq_ty_denote:
-  "ty_eq \<Gamma> t t' k \<Longrightarrow> ty_denote \<sigma> t = ty_denote \<sigma> t'"
-apply (induct arbitrary: \<sigma> set: ty_eq)
-apply simp (* refl *)
-apply simp (* sym *)
-apply simp (* trans *)
-apply simp (* TyApp *)
-apply simp (* TyAll *)
-apply (drule ty_ax_ty_denote, simp) (* axiom *)
+lemma steps_ty_denote:
+  "steps t u \<Longrightarrow> ty_denote \<sigma> t = ty_denote \<sigma> u"
+apply (induct set: steps)
+apply simp (* Why does "rule refl" fail? *)
+apply (auto dest: step_ty_denote)
+done
+
+lemma conv_ty_denote:
+  "conv t u \<Longrightarrow> ty_denote \<sigma> t = ty_denote \<sigma> u"
+apply (induct set: conv)
+apply (erule trans [OF steps_ty_denote])
+apply (erule sym [OF steps_ty_denote])
 done
 
 end
